Word.v
@@ -1,0 +1,35 @@
+Require Import Coqlib.
+Require Import Integers.
+
+Definition byte := byte.
+
+Module Wordsize_256.
+  Definition wordsize := 256%nat.
+  Remark wordsize_not_zero: wordsize <> 0%nat.
+  Proof. unfold wordsize; congruence. Qed.
+End Wordsize_256.
+
+Strategy opaque [Wordsize_256.wordsize].
+
+Module Int256.
+
+Include Make(Wordsize_256).
+End Int256.
+
+Notation int256 := Int256.int.
+
+Module Word := Int256.
+Definition word := Word.int.
+
+Import Word.
+
+Definition shl8 (w : word) := shl w (repr 8).
+
+Definition conc (w1 : word) (b : byte) :=  repr ((unsigned (shl8 w1)) + (Byte.unsigned b)).
+
+Notation "a @ b" := (conc a b) (at level 1).
+
+Definition word_from_bytes (a1 a2 a3 a4 a5 a6 a7 a8 : byte) : word :=
+  zero @ a1 @ a2 @ a3 @ a4 @ a5 @ a6 @ a7 @ a8.
+
+Axiom bytes_from_word : word -> byte*byte*byte*byte*byte*byte*byte*byte.
